Tweaks necessary in `Subst`

theories/Partition.v
@@ -11,151 +11,139 @@ From Lang Require Import
 
 (* Partition a context into types (which allow structural rules) and values (which don't). *)
 Inductive Partition {T} : list T -> list T -> list T -> Prop :=
-  | PartitionDone : forall src,
-      Partition src [] src
-  | PartitionCpHi : forall x src hi lo,
-      In x hi ->
-      Partition src hi lo ->
-      Partition src (x :: hi) lo
-  | PartitionCpLo : forall x src hi lo,
-      ~In x hi ->
+  | PartitionDone : forall lo,
+      Partition [] [] lo
+  | PartitionCpLo : forall x pf hi lo,
       In x lo ->
-      Partition src hi lo ->
-      Partition src (x :: hi) lo
-  | PartitionMove : forall x src hi lo,
+      Partition pf hi lo ->
+      Partition pf (x :: hi) lo
+  | PartitionCpPf : forall x pf hi lo,
+      ~In x lo ->
+      In x pf ->
+      In x hi ->
+      Partition pf hi lo ->
+      Partition pf (x :: hi) lo
+  | PartitionMove : forall x pf hi lo,
+      ~In x lo ->
+      ~In x pf ->
       ~In x hi ->
-      ~In x src ->
-      Partition src hi lo ->
-      Partition (x :: src) (x :: hi) lo
+      Partition pf hi lo ->
+      Partition (x :: pf) (x :: hi) lo
   .
-Arguments Partition {T} src hi lo.
+Arguments Partition {T} pf hi lo.
 Ltac partition_done := apply PartitionDone.
-Ltac partition_copy_hi := eapply PartitionCpHi; [auto_in |].
-Ltac partition_copy_lo := eapply PartitionCpLo; [intros C; not_in C | auto_in |].
-Ltac partition_move := eapply PartitionMove; [intros C; not_in C | intros C; not_in C |].
-Ltac partition_step := first [partition_done | partition_copy_hi | partition_copy_lo | partition_move].
+Ltac partition_copy_lo := eapply PartitionCpLo; [auto_in |].
+Ltac partition_copy_pf := eapply PartitionCpPf; [intros C; not_in C | auto_in | auto_in |].
+Ltac partition_move := eapply PartitionMove; [intros C; not_in C | intros C; not_in C | intros C; not_in C |].
+Ltac partition_step := first [partition_done | partition_copy_lo | partition_copy_pf | partition_move].
 Ltac try_partition := repeat partition_step.
-Ltac partition := first [partition_done | first [partition_copy_hi | partition_copy_lo | partition_move]; partition].
+Ltac partition := first [partition_done | first [partition_copy_lo | partition_copy_pf | partition_move]; partition].
 
-Example partition_12345 : Partition [4;2;1;3;5] [1;1;1;1;1;1;4;2;3;2;2;3] [1;3;5]. Proof. partition. Qed.
+Example partition_12345 : Partition [4;2] [1;1;1;1;1;1;4;2;3;2;2;3] [1;3;5]. Proof. partition. Qed.
 
-Theorem partition_src_app_lo : forall {T} src hi lo,
-  @Partition T src hi lo ->
-  exists pre, src = pre ++ lo.
+Theorem partition_deterministic : forall {T} pf pf' hi lo,
+  @Partition T pf hi lo ->
+  Partition pf' hi lo ->
+  pf = pf'.
 Proof.
-  intros. induction H.
-  - exists []. reflexivity.
-  - apply IHPartition.
-  - apply IHPartition.
-  - destruct IHPartition as [pre E]. exists (x :: pre). simpl. f_equal. assumption.
-Qed.
-
-Theorem partition_deterministic : forall {T} src src' hi lo,
-  @Partition T src hi lo ->
-  Partition src' hi lo ->
-  src = src'.
-Proof.
-  intros. generalize dependent src'. induction H; intros; simpl in *.
+  intros. generalize dependent pf'. induction H; intros; simpl in *.
   - invert H0. reflexivity.
   - invert H1.
     + apply IHPartition; assumption.
     + apply H4 in H as [].
     + apply H4 in H as [].
-  - invert H2.
-    + apply H in H6 as [].
-    + apply IHPartition; assumption.
-    + apply partition_src_app_lo in H9 as [pre E]. subst. rewrite in_app_iff in H7.
-      apply Decidable.not_or in H7 as [H2 H3]. apply H3 in H0 as [].
-  - invert H2.
-    + apply H in H6 as [].
-    + apply partition_src_app_lo in H1 as [pre E]. subst. rewrite in_app_iff in H0.
-      apply Decidable.not_or in H0 as [H2 H3]. apply H3 in H7 as [].
-    + f_equal. apply IHPartition; assumption.
+  - invert H3.
+    + apply H in H7 as [].
+    + apply IHPartition. assumption.
+    + apply H9 in H1 as [].
+  - invert H3.
+    + apply H in H7 as [].
+    + apply H1 in H9 as [].
+    + f_equal. apply IHPartition. assumption.
 Qed.
 
-(* not efficient at all but not a problem right now *)
-Fixpoint partition_src_with {T} (f : T -> T -> bool) hi lo :=
+Fixpoint partition_pf_slow {T} f (hi lo : list T) :=
   match hi with
-  | [] => lo
+  | [] => []
   | hd :: tl =>
-      let recursed := partition_src_with f tl lo in
-      (* NOTE: Checking for existence in `recursed` checks both `lo` AND `tl` at once. *)
-      if existsb (f hd) recursed then recursed else hd :: recursed
+      let recursed := partition_pf_slow f tl lo in
+      if (existsb (f hd) lo || existsb (f hd) tl)%bool then recursed else hd :: recursed
   end.
 
-Theorem count_partition_src : forall {T} x f hi lo,
+Fixpoint partition_pf_fast {T} acc f (hi lo : list T) :=
+  match hi with
+  | [] => acc
+  | hd :: tl =>
+      partition_pf_fast (if (existsb (f hd) lo || existsb (f hd) tl)%bool then acc else hd :: acc) f tl lo
+  end.
+Definition partition_pf {T} f hi lo := rev' (@partition_pf_fast T [] f hi lo).
+Arguments partition_pf {T}/ f hi lo.
+
+Theorem partition_pf_fast_acc : forall {T} hd tl f hi lo,
+  @partition_pf_fast T (hd ++ tl) f hi lo = partition_pf_fast hd f hi lo ++ tl.
+Proof.
+  intros T hd tl f hi. generalize dependent hd. generalize dependent tl. generalize dependent f.
+  induction hi; intros; simpl in *. { reflexivity. }
+  destruct (existsb (f a) lo); simpl in *. { apply IHhi. }
+  destruct (existsb (f a) hi); simpl in *. { apply IHhi. }
+  apply (IHhi _ tl (a :: hd)).
+Qed.
+
+Theorem partition_pf_fast_slow : forall {T} f hi lo,
+  @partition_pf T f hi lo = partition_pf_slow f hi lo.
+Proof.
+  intros T f hi. generalize dependent f. induction hi; intros; simpl in *. { reflexivity. }
+  destruct (existsb (f a) lo); simpl in *. { apply IHhi. }
+  destruct (existsb (f a) hi); simpl in *. { apply IHhi. }
+  rewrite (partition_pf_fast_acc [] [a]). unfold rev'. rewrite <- rev_alt. rewrite rev_app_distr. simpl.
+  f_equal. rewrite rev_alt. apply IHhi.
+Qed.
+
+Theorem in_partition_pf : forall {T} x f hi lo,
   (forall a b : T, Bool.reflect (a = b) (f a b)) ->
-  count f x (partition_src_with f hi lo) = (
-    match count f x lo with
-    | O =>
-        match count f x hi with
-        | O => O
-        | S _ => 1
-        end
-    | S n =>
-        S n
-    end).
+  In x (partition_pf f hi lo) <-> (In x hi /\ ~In x lo).
 Proof.
-  intros. generalize dependent x. generalize dependent f. generalize dependent lo.
-  induction hi; intros; simpl in *. { destruct (count_acc 0 f x lo); reflexivity. }
-  destruct (count_existsb f a (partition_src_with f hi lo) X); simpl in *.
-  - destruct (X x a); [| apply IHhi; apply X]. rewrite count_S. subst. simpl in *.
-    destruct (count_acc 0 f a (partition_src_with f hi lo)) eqn:Ep. { contradiction n. reflexivity. } clear n.
-    rewrite IHhi in Ep; [| apply X]. destruct (count_acc 0 f a lo) eqn:El; [| symmetry; assumption].
-    destruct (count_acc 0 f a hi). { discriminate Ep. } symmetry. assumption.
-  - destruct (X x a); [| apply IHhi; apply X]. subst. repeat rewrite count_S.
-    destruct (count_acc 0 f a (partition_src_with f hi lo)) eqn:Ep; [| contradiction n; intro C; discriminate C]. clear n.
-    rewrite IHhi in Ep; [| apply X]. destruct (count_acc 0 f a lo); [| discriminate Ep]. reflexivity.
+  split; intros; rewrite partition_pf_fast_slow in *.
+  - generalize dependent x. generalize dependent f. generalize dependent lo.
+    induction hi; intros; simpl in *. { destruct H. }
+    destruct (existsb_in f a lo X). { apply (IHhi _ _ X) in H as [Hh Hl]. split; [right |]; assumption. }
+    destruct (existsb_in f a hi X). { apply (IHhi _ _ X) in H as [Hh Hl]. split; [right |]; assumption. }
+    destruct H. { subst. split. { left. reflexivity. } assumption. }
+    apply (IHhi _ _ X) in H as [Hh Hl]. split; [right |]; assumption.
+  - destruct H as [Hh Hl]. generalize dependent x. generalize dependent f. generalize dependent lo.
+    induction hi; intros; simpl in *; destruct Hh; [symmetry in H; subst |];
+    (destruct (existsb_in f a lo X); [apply (IHhi _ _ X); auto; apply Hl in i as [] |]);
+    (destruct (existsb_in f a hi X); [apply (IHhi _ _ X); assumption |]). { left. reflexivity. }
+    simpl. destruct (X a x). { left. assumption. } right. apply (IHhi _ _ X); assumption.
 Qed.
 
-Theorem existsb_partition_src : forall {T} x f hi lo,
+Lemma incl_partition_pf : forall {T} f hi lo,
   (forall a b : T, Bool.reflect (a = b) (f a b)) ->
-  existsb (f x) (partition_src_with f hi lo) = orb (existsb (f x) hi) (existsb (f x) lo).
+  incl (partition_pf f hi lo) hi.
+Proof. unfold incl. intros. apply (in_partition_pf _ _ _ _ X) in H as [Hh Hl]. assumption. Qed.
+
+Theorem partition_pf_works : forall {T} f hi lo,
+  (forall a b : T, Bool.reflect (a = b) (f a b)) ->
+  Partition (partition_pf f hi lo) hi lo.
 Proof.
-  intros. destruct (count_existsb f x (partition_src_with f hi lo) X);
-  destruct (count_existsb f x hi X); destruct (count_existsb f x lo X);
-  try reflexivity; rewrite count_partition_src in n; destruct (count f x hi); auto; destruct (count f x lo); lia.
+  intros. rewrite partition_pf_fast_slow. generalize dependent f. generalize dependent lo.
+  induction hi; intros; simpl in *. { constructor. }
+  destruct (existsb_in f a lo X). { apply PartitionCpLo; [assumption | apply (IHhi _ _ X)]. }
+  destruct (existsb_in f a hi X). {
+    apply PartitionCpPf; [assumption | | assumption | apply (IHhi _ _ X)].
+    rewrite <- partition_pf_fast_slow. apply (in_partition_pf _ _ _ _ X). split; assumption. }
+  apply PartitionMove; [assumption | | assumption | apply (IHhi _ _ X)].
+  intro C. rewrite <- partition_pf_fast_slow in C.
+  apply (in_partition_pf _ _ _ _ X) in C as [Hh Hl]. apply n0 in Hh as [].
 Qed.
 
-Theorem in_partition_src : forall {T} x (f : T -> T -> bool) hi lo,
+Theorem reflect_partition_pf : forall {T} (f : T -> T -> bool) pf hi lo,
   (forall a b, Bool.reflect (a = b) (f a b)) ->
-  In x (partition_src_with f hi lo) <-> (In x hi \/ In x lo).
-Proof.
-  intros. repeat (rewrite existsb_in_iff; [| apply X]).
-  rewrite existsb_partition_src; [| apply X]. apply Bool.orb_true_iff.
-Qed.
-
-Theorem not_in_partition_src : forall {T} x (f : T -> T -> bool) hi lo,
-  (forall a b, Bool.reflect (a = b) (f a b)) ->
-  ~In x (partition_src_with f hi lo) <-> (~In x hi /\ ~In x lo).
-Proof.
-  intros. repeat (rewrite existsb_in_iff; [| apply X]).
-  rewrite existsb_partition_src; [| apply X].
-  repeat rewrite Bool.not_true_iff_false. apply Bool.orb_false_iff.
-Qed.
-
-Theorem partition_src_works : forall {T} (f : T -> T -> bool) hi lo,
-  (forall a b, Bool.reflect (a = b) (f a b)) ->
-  Partition (partition_src_with f hi lo) hi lo.
-Proof.
-  intros. generalize dependent f. generalize dependent lo. induction hi; intros; simpl in *. { constructor. }
-  destruct (existsb_in f a (partition_src_with f hi lo) X).
-  - rewrite in_partition_src in i; [| apply X]. destruct i.
-    + apply PartitionCpHi; [| apply IHhi]; assumption.
-    + destruct (existsb_in f a hi X).
-      * apply PartitionCpHi; [| apply IHhi]; assumption.
-      * apply PartitionCpLo; [| | apply IHhi]; assumption.
-  - apply not_in_partition_src in n as [Hhi Hlo]; [| apply X]. apply PartitionMove; [assumption | | apply IHhi; assumption].
-    intro C. apply in_partition_src in C as [C | C]; [| | assumption]. { apply Hhi in C as []. } apply Hlo in C as [].
-Qed.
-
-Theorem reflect_partition_src : forall {T} (f : T -> T -> bool) src hi lo,
-  (forall a b, Bool.reflect (a = b) (f a b)) ->
-  (partition_src_with f hi lo = src <-> Partition src hi lo).
+  (partition_pf f hi lo = pf <-> Partition pf hi lo).
 Proof.
   split; intros.
-  - subst. apply partition_src_works. assumption.
-  - eapply partition_deterministic. { apply partition_src_works. assumption. } assumption.
+  - subst. apply partition_pf_works. assumption.
+  - eapply partition_deterministic. { apply partition_pf_works. assumption. } assumption.
 Qed.
 
 Definition ap_fst {A B C} : (A -> C) -> ((A * B) -> C) := fun f x => let (a, b) := x in f a.
@@ -168,24 +156,24 @@ Proof.
   destruct a. simpl. rewrite H. destruct (f' x a). { reflexivity. } apply IHli. assumption.
 Qed.
 
-Lemma map_fst_partition_src : forall {A B} f f' hi lo,
+Lemma map_fst_partition_pf : forall {A B} f f' hi lo,
   (forall (a a' : A) (b b' : B), f (a, b) (a', b') = f' a a') ->
-  map fst (partition_src_with f hi lo) = partition_src_with f' (map fst hi) (map fst lo).
+  map fst (partition_pf f hi lo) = partition_pf f' (map fst hi) (map fst lo).
 Proof.
-  intros. generalize dependent lo. generalize dependent f'. generalize dependent f.
+  intros. repeat rewrite partition_pf_fast_slow. generalize dependent lo. generalize dependent f'. generalize dependent f.
   induction hi; intros; simpl in *. { reflexivity. }
-  destruct a. simpl. rewrite (existsb_map_fst _ f f' _ _ H). rewrite (IHhi _ _ H).
-  destruct (existsb (f' a) (partition_src_with f' (map fst hi) (map fst lo))) eqn:E.
-  - apply IHhi. assumption.
-  - simpl. f_equal. apply IHhi. assumption.
+  destruct a as [a b]. simpl in *. repeat rewrite (existsb_map_fst _ f f' _ _ H).
+  destruct (existsb (f' a) (map fst lo)). { apply (IHhi _ _ H). }
+  destruct (existsb (f' a) (map fst hi)). { apply (IHhi _ _ H). }
+  simpl. f_equal. apply (IHhi _ _ H).
 Qed.
 
 Theorem partition_map_fst : forall {A B} f f' hi lo,
   (forall a b : A, Bool.reflect (a = b) (f' a b)) ->
   (forall (a a' : A) (b b' : B), f (a, b) (a', b') = f' a a') ->
-  Partition (map fst (partition_src_with f hi lo)) (map fst hi) (map fst lo).
+  Partition (map fst (partition_pf f hi lo)) (map fst hi) (map fst lo).
 Proof.
-  intros. erewrite map_fst_partition_src. { apply partition_src_works. apply X. } assumption.
+  intros. erewrite map_fst_partition_pf. { apply partition_pf_works. apply X. } assumption.
 Qed.
 
 Definition fst_cmp {A B} := fun (a : string * A) (b : string * B) => eqb (fst a) (fst b).
@@ -196,30 +184,4 @@ Proof.
   intros T li. induction li; intros; simpl in *. { reflexivity. }
   destruct a. unfold fst_cmp. simpl in *. destruct (eqb s s0). { reflexivity. }
   apply (IHli _ t).
-Qed.
-
-Fixpoint set_diff {T} (a b : list (string * T)) :=
-  match a with
-  | [] => []
-  | hd :: tl =>
-      let recursed := set_diff tl b in
-      if (existsb (fst_cmp hd) tl || existsb (fst_cmp hd) b)%bool then recursed else hd :: recursed
-  end.
-
-Theorem incl_set_diff : forall {T} (a b : list (string * T)),
-  incl (set_diff a b) a.
-Proof.
-  unfold incl. induction a; intros; simpl in *. { destruct H. }
-  destruct (existsb (fst_cmp a) a0) eqn:Ea; simpl in *. { right. eapply IHa. apply H. }
-  destruct (existsb (fst_cmp a) b) eqn:Eb; simpl in *. { right. eapply IHa. apply H. }
-  destruct H. { left. assumption. } right. eapply IHa. apply H.
-Qed.
-
-Theorem partition_src_app : forall {T} (a b : list (string * T)),
-  partition_src_with fst_cmp a b = set_diff a b ++ b.
-Proof.
-  induction a; intros; simpl in *. { reflexivity. }
-  destruct a. repeat rewrite has_cmp_fst. erewrite map_fst_partition_src;
-  [| intros; unfold fst_cmp; simpl; reflexivity]. rewrite (existsb_partition_src _ _ _ _ eqb_spec).
-  destruct (existsb (eqb s) (map fst a0) || existsb (eqb s) (map fst b))%bool; simpl; f_equal; apply IHa.
 Qed.
